examples/ring/RingIAproof.v
@@ -1,0 +1,161 @@
+Require Import Coqlib ITreelib sflib.
+Require Import SMod ModSim.
+Require Import ImpPrelude.
+Require Import Skeleton.
+Require Import PCM IPM IFacts.
+Require Import Events Behavior.
+Require Import Relation_Definitions.
+
+(*** TODO: export these in Coqlib or Universe ***)
+Require Import Relation_Operators.
+Require Import RelationPairs.
+From ITree Require Import
+     Events.MapDefault.
+From ExtLib Require Import
+     Core.RelDec
+     Structures.Maps
+     Data.Map.FMapAList.
+Require Import Mem1 STB.
+
+Require Import ISim HMod Events.
+Require Import Mod ModSimFacts.
+Require Import CellHeader CellASpec CellA RingHeader RingA RingASpec CtrlI.
+
+Set Implicit Arguments.
+
+Local Open Scope nat_scope.
+
+Module RingIA.
+Section SIMMODSEM.
+  Context `{Σ: GRA.t}.
+  Context `{_M: CellRA.t (Σ:=Σ)}.
+
+  Variable max_size : nat.
+
+  Variable StbA: Sk.t -> gname -> option fspec.
+  Hypothesis RingInStb: forall sk, stb_incl (to_stb RingAS.Stb) (StbA sk).
+  Hypothesis CellInStb: forall sk idx (LT: idx < max_size), stb_incl (to_stb (CellAS.Stb idx)) (StbA sk).
+
+  Import CellAS.
+
+  Local Notation RingAMod := (RingA.t max_size StbA).
+  Local Notation CtrlIMod := (CtrlI.t max_size).
+  Local Notation CellAMod := (fun i => CellA.t max_size StbA).
+
+  Variable HMod_empty: HMod.t.
+
+  Fixpoint CellGroup (i: nat) : HMod.t :=
+    match i with
+    | 0 => HMod_empty
+    | S i' => HMod.add (CellAMod i') (CellGroup i')
+    end.
+
+  Local Notation RingIMod := (HMod.add CtrlIMod (CellGroup max_size)).
+
+  Print rotate.
+
+  Definition rotate_rev {T} n (l: list T) :=
+    drop ((strings.length l)-(n mod strings.length l)) l ++ take ((strings.length l)-(n mod strings.length l)) l.
+
+  Lemma rotate_rev_inv {T} n (l: list T):
+    rotate_rev n (rotate n l) = l.
+  Proof. admit. Admitted.
+
+  Lemma rotate_rev_id {T} (l: list T):
+    rotate_rev 0 l = l.
+  Proof. admit. Admitted.
+  
+  Definition Ist: Any.t -> Any.t -> iProp :=
+    (fun st_src st_tgt =>
+       ((∃ (sz:nat) (q q': list Z) (hd tl: nat) cell_state,
+         ⌜st_src = (sz, q)↑ /\ List.length q = sz /\ sz < max_size /\
+          st_tgt = Any.pair (hd,tl)↑ cell_state /\ hd-tl = sz /\
+          List.length (q ++ q') = max_size⌝ ∗
+          [∗ list] i↦x ∈ rotate_rev tl (q++q'), (CellAS.pending i ∨ CellAS.cell (i mod max_size) x))))%I.
+
+  Variable fl: alist string (Any.t → itree hmodE Any.t).
+  Variable fr: alist string (Any.t → itree hmodE Any.t).
+  
+  Lemma simF_init:
+    HModR.sim_fun RingAMod RingIMod Ist RingName.init.
+  Proof.
+    cut (forall sk, isim_fsem Ist fl fr
+     (λ '(st_src0, v_src) '(st_tgt0, v_tgt), Ist st_src0 st_tgt0 ** ⌜v_src = v_tgt⌝)
+     (interp_sb_hp (StbA sk) {| fsb_fspec := fspec_trivial; fsb_body :=  cfunU RingA.init |})
+     (fun args => translate (HModSem.emb_ run_l) (cfunU CtrlI.init args))).
+    { admit. }
+    unfold interp_sb_hp, HoareFun, cfunU, ccallU; s;
+    unfold RingA.init, CtrlI.init.
+    ii; subst; iIntros "IST".
+
+    (* init_simF. *)
+
+    st_l. iDestruct "ASM" as "%". subst. hss.
+
+    st_r. force_l. st_l. force_l.
+    iSplitL "". { eauto. }
+
+    st.
+    iSplitL; eauto. unfold Ist.
+    iDestruct "IST" as (sz q q' hd tl cell_state) "(% & CS)".
+    des; subst.
+    iExists 0, [], (rotate_rev tl (q++q')%list), 0, 0, cell_state. s.
+    replace (rotate_rev 0 (rotate_rev tl (q ++ q'))) with
+      (rotate_rev tl (q ++ q')) by admit.
+    iFrame. hss.
+    iPureIntro. esplits; eauto; try nia.
+    admit.
+  Admitted.
+
+  Lemma simF_get:
+    HModR.sim_fun CellAMod CellIMod Ist (CellName.get idx).
+  Proof.
+    init_simF.
+
+    st_l. iDestruct "ASM" as "((% & C) & %)".
+    subst. hss. rename y0 into v. unfold Ist.
+    iDestruct "IST" as "[(C0 & _)|(P & IST)]".
+    { iExFalso. iApply (cell_unique with "C0 C"). }
+    iDestruct "IST" as (v') "(A & %)". subst. hss.
+
+    iPoseProof (cell_auth_get with "C A") as "%". subst.
+
+    st_r. force_l. st_l. force_l. force_l.
+    iSplitL "C". { eauto. }
+
+    st. iSplitL; [|eauto].
+    iRight. iFrame. eauto.
+  Qed.
+  
+  Lemma simF_set:
+    HModR.sim_fun CellAMod CellIMod Ist (CellName.set idx).
+  Proof.
+    init_simF.
+    
+    st_l. hss. iDestruct "ASM" as "((% & C) & %)".
+    subst. hss. rename y1 into v, y2 into v0. unfold Ist.
+    iDestruct "IST" as "[(C0 & _)|(P & IST)]".
+    { iExFalso. iApply (cell_unique with "C0 C"). }
+    iDestruct "IST" as (v') "(A & %)". subst. hss.
+
+    iPoseProof (cell_auth_get with "C A") as "%". subst.
+    iMod (cell_auth_set with "C A") as "(C & A)".
+    
+    st_r. force_l. st_l. force_l. force_l.
+    iSplitL "C". { eauto. }
+
+    st. iSplitL; [|eauto].
+    iRight. iFrame. eauto.
+  Qed.
+
+  Theorem sim: HModR.sim CellAMod CellIMod Ist.
+  Proof.
+    init_sim.
+    - unfold Ist. eauto.
+    - use_simF simF_init.
+    - use_simF simF_get.
+    - use_simF simF_set.
+  Qed.
+
+End SIMMODSEM.
+End RingIA.
